Preservation_.v
@@ -1,0 +1,23 @@
+From Elo Require Import Core.
+
+Ltac simpl_forall := 
+  match goal with
+  | |- forall_threads _[_ <- _] _          => intros tid'; Array.sgs
+  | |- forall_threads (_[_ <- _] +++ _) _  => intros tid'; Array.sgas
+  end.
+
+Ltac destruct_forall_program :=
+  progress (repeat (
+    match goal with H : forall_program _ _ _ |- _ => destruct H end
+  )).
+
+Ltac split_preservation := 
+  intros;
+  match goal with
+  (* vad | ctr | ss *)
+  | H : forall_program ?m1 ?ths1 (?P ?m1),
+    _ : ?m1 / ?ths1 ~~[_, _]~~> ?m2 / ?ths2
+     |- forall_program ?m2 ?ths2 (?P ?m2) =>
+    destruct_forall_program;
+    invc_cstep; try invc_mstep; trivial; split; try simpl_forall; trivial
+  end.
