SimpleLemmas.v
@@ -5,48 +5,9 @@ From Elo Require Import Properties.
 (*                                                                           *)
 (* ------------------------------------------------------------------------- *)
 
-Lemma empty_eq_safe_empty :
-  empty = safe empty.
-Proof.
-  eauto.
-Qed.
 
 (* ------------------------------------------------------------------------- *)
 (*                                                                           *)
 (* ------------------------------------------------------------------------- *)
 
-Lemma ctr_tstep_alloc_term : forall m t1 t2 ad t T,
-  consistently_typed_references m t1 ->
-  t1 --[e_alloc ad t T ]--> t2 ->
-  consistently_typed_references m t.
-Proof.
-  intros. ind_tstep; inv_ctr; eauto using consistently_typed_references.
-Qed.
-
-Lemma ctr_tstep_write_term : forall m t1 t2 ad t T,
-  consistently_typed_references m t1 ->
-  t1 --[e_write ad t T ]--> t2 ->
-  consistently_typed_references m t.
-Proof.
-  intros. ind_tstep; inv_ctr; eauto.
-Qed.
-
-(* ------------------------------------------------------------------------- *)
-(*                                                                           *)
-(* ------------------------------------------------------------------------- *)
-
-Lemma consistently_typed_write_effect : forall m t1 t2 ad t T,
-  well_typed_term t1 ->
-  consistently_typed_references m t1 ->
-  (* --- *)
-  t1 --[e_write ad t T]--> t2 ->
-  exists Tm, T = `w&Tm`
-          /\ empty |-- t is Tm
-          /\ empty |-- m[ad].tm is Tm
-          /\ m[ad].ty = `w&Tm`.
-Proof.
-  intros * [T' ?] **. generalize dependent T'.
-  ind_tstep; intros; inv_typeof; inv_ctr; eauto.
-  inv_typeof. inv_ctr. eauto.
-Qed.
 
