ValidPointerTypes.v
@@ -1,0 +1,149 @@
+From Coq Require Import Lia.
+
+From Elo Require Import Core.
+
+From Elo Require Import WellTypedTerm.
+
+(* ------------------------------------------------------------------------- *)
+(* well-typed-memory                                                         *)
+(* ------------------------------------------------------------------------- *)
+
+Reserved Notation " T1 '~>' T2  " (at level 80, no associativity).
+
+Inductive points_to_type : ty -> ty -> Prop :=
+  | pt_R : forall T,
+    `r&T` ~> `Safe T`
+
+  | pt_X : forall T,
+    `x&T` ~> T
+
+  | pt_W : forall T,
+    `w&T` ~> T
+
+  where "T1 ~> T2" := (points_to_type T1 T2).
+
+Definition valid_pointer_types (m : mem) :=
+  forall ad T, ad < #m -> empty |-- m[ad].tm is T -> m[ad].ty ~> T.
+
+(* ------------------------------------------------------------------------- *)
+(* preservation                                                              *)
+(* ------------------------------------------------------------------------- *)
+
+Local Lemma deterministic_R : forall t T1 T2,
+  empty |-- t is `Safe T1` ->
+  empty |-- t is T2 ->
+  `r&T1` ~> T2.
+Proof.
+  intros.
+  assert (`Safe T1` = T2) by eauto using deterministic_typing.
+  subst. eauto using points_to_type.
+Qed.
+
+Local Lemma deterministic_X : forall t T1 T2,
+  empty |-- t is T1 ->
+  empty |-- t is T2 ->
+  `x&T1` ~> T2.
+Proof.
+  intros.
+  assert (T1 = T2) by eauto using deterministic_typing.
+  subst. eauto using points_to_type.
+Qed.
+
+Local Lemma deterministic_W : forall t T1 T2,
+  empty |-- t is T1 ->
+  empty |-- t is T2 ->
+  `w&T1` ~> T2.
+Proof.
+  intros.
+  assert (T1 = T2) by eauto using deterministic_typing.
+  subst. eauto using points_to_type.
+Qed.
+
+Local Lemma vpt_acq_rel : forall m otid ad t T,
+  valid_pointer_types m ->
+  empty |-- t is T ->
+  ad < # m ->
+  m[ad].tm = <{ptm otid t}> ->
+  m[ad].ty ~> T.
+Proof.
+  intros * Hvpt ? ? Heq.
+  eapply Hvpt; trivial.
+  rewrite Heq. eauto using type_of.
+Qed.
+
+(* ------------------------------------------------------------------------- *)
+
+Lemma vpt_preservation_alloc : forall m t1 t2 t T,
+  well_typed_term t1 ->
+  (* --- *)
+  valid_pointer_types m ->
+  t1 --[e_alloc (#m) t T]--> t2 ->
+  valid_pointer_types (m +++ (t, T)).
+Proof.
+  intros * [T' ?] **. generalize dependent T'.
+  ind_tstep; intros; invc_typeof; eauto;
+  intros ? ? ? ?; Array.sga; simpl in *; eauto; Array.simpl_lengths; try lia;
+  try invc_typeof;
+  eauto using deterministic_R, deterministic_X, deterministic_W.
+Qed.
+
+Lemma vpt_preservation_write : forall m t1 t2 ad t T,
+  well_typed_term t1 ->
+  (* --- *)
+  valid_pointer_types m ->
+  t1 --[e_write ad t T]--> t2 ->
+  valid_pointer_types m[ad <- (t, T)].
+Proof.
+  intros * [T' ?] **. generalize dependent T'.
+  ind_tstep; intros; invc_typeof; eauto.
+  intros ? ? ? ?. invc_typeof. 
+  Array.simpl_lengths. Array.sgs; eauto using deterministic_W.
+Qed.
+
+Lemma vpt_preservation_acq : forall m t1 t2 otid1 otid2 tid ad t,
+  well_typed_term t1 ->
+  (* --- *)
+  m[ad].tm = <{ptm otid1 t}> ->
+  valid_pointer_types m ->
+  t1 --[e_acq tid ad t]--> t2 ->
+  valid_pointer_types m[ad <- (<{ptm otid2 t}>, m[ad].ty)].
+Proof.
+  intros * [T' ?] **. generalize dependent T'.
+  ind_tstep; intros; invc_typeof; eauto.
+  intros ? ? ? ?. repeat invc_typeof.
+  Array.simpl_lengths. Array.sgs; eauto.
+  simpl in *. invc_typeof. eauto using vpt_acq_rel.
+Qed.
+
+Lemma vpt_preservation_rel : forall m t1 t2 otid1 otid2 tid ad t,
+  well_typed_term t1 ->
+  (* --- *)
+  m[ad].tm = <{ptm otid1 t}> ->
+  valid_pointer_types m ->
+  t1 --[e_rel tid ad]--> t2 ->
+  valid_pointer_types m[ad <- (<{ptm otid2 t}>, m[ad].ty)].
+Proof.
+  intros * [T' ?] **. generalize dependent T'.
+  ind_tstep; intros; invc_typeof; eauto.
+  intros ? ? ? ?.
+  Array.simpl_lengths. Array.sgs; eauto.
+  simpl in *. invc_typeof. eauto using vpt_acq_rel.
+Qed.
+
+(* ------------------------------------------------------------------------- *)
+
+Theorem vpt_preservation : forall m1 m2 ths1 ths2 tid e,
+  forall_program m1 ths1 well_typed_term ->
+  (* --- *)
+  valid_pointer_types m1 ->
+  m1 / ths1 ~~[tid, e]~~> m2 / ths2 ->
+  valid_pointer_types m2.
+Proof.
+  intros * Hwtt **. invc Hwtt.
+  invc_cstep; try invc_mstep;
+  eauto using vpt_preservation_alloc,
+              vpt_preservation_write,
+              vpt_preservation_acq,
+              vpt_preservation_rel.
+Qed.
+
