WellTypedTerm.v
@@ -1,0 +1,92 @@
+From Elo Require Import Core.
+
+(* ------------------------------------------------------------------------- *)
+(* well-typed-term                                                           *)
+(* ------------------------------------------------------------------------- *)
+
+Definition well_typed_term (t : tm) :=
+  exists T, empty |-- t is T.
+
+(* ------------------------------------------------------------------------- *)
+(* tactics                                                                   *)
+(* ------------------------------------------------------------------------- *)
+
+Local Ltac solve_wtt_inversion := 
+  intros * [? ?]; try split;
+  inv_typeof; try discriminate; eauto; eexists; eauto.
+
+Local Lemma inv_wtt_var : forall x,
+  well_typed_term <{var x}> ->
+  False.
+Proof. solve_wtt_inversion. Qed.
+
+Local Lemma inv_wtt_fun : forall x Tx t,
+  well_typed_term <{fn x Tx t}> ->
+  exists T, empty[x <== Tx] |-- t is T.
+Proof. solve_wtt_inversion. Qed.
+
+Local Lemma inv_wtt_call : forall t1 t2,
+  well_typed_term <{call t1 t2}> ->
+  well_typed_term t1 /\ well_typed_term t2.
+Proof. solve_wtt_inversion. Qed.
+
+Local Lemma inv_wtt_ref : forall ad T,
+  well_typed_term <{&ad : T}> ->
+    (exists T', T = `r&T'`) \/
+    (exists T', T = `x&T'`) \/
+    (exists T', T = `w&T'`).
+Proof. solve_wtt_inversion. Qed.
+
+Local Lemma inv_wtt_new : forall t T,
+  well_typed_term <{new t : T}> ->
+  well_typed_term t.
+Proof. solve_wtt_inversion. Qed.
+
+Local Lemma inv_wtt_load : forall t,
+  well_typed_term <{*t}> ->
+  well_typed_term t.
+Proof. solve_wtt_inversion. Qed.
+
+Local Lemma inv_wtt_asg : forall t1 t2,
+  well_typed_term <{t1 := t2}> ->
+  well_typed_term t1 /\ well_typed_term t2.
+Proof. solve_wtt_inversion. Qed.
+
+Local Lemma inv_wtt_acq : forall t1 t2,
+  well_typed_term <{acq t1 t2}> ->
+  well_typed_term t1 /\ well_typed_term t2.
+Proof. solve_wtt_inversion. Qed.
+
+Local Lemma inv_wtt_cr : forall ad t,
+  well_typed_term <{cr ad t}> ->
+  well_typed_term t.
+Proof. solve_wtt_inversion. Qed.
+
+Local Lemma inv_wtt_ptm : forall otid t,
+  well_typed_term <{ptm otid t}> ->
+  well_typed_term t.
+Proof. solve_wtt_inversion. Qed.
+
+Local Lemma inv_wtt_spawn : forall t,
+  well_typed_term <{spawn t}> ->
+  well_typed_term t.
+Proof. solve_wtt_inversion. Qed.
+
+Local Notation wtt := (well_typed_term ).
+
+Ltac invc_wtt :=
+  match goal with
+  (* irrelevant for unit and nat *)
+  | H : wtt <{var _    }> |- _ => eapply inv_wtt_var   in H; contradiction
+  | H : wtt <{fn _ _ _ }> |- _ => eapply inv_wtt_fun   in H as [? ?]
+  | H : wtt <{call _ _ }> |- _ => eapply inv_wtt_call  in H as [? ?]
+  | H : wtt <{& _ : _  }> |- _ => eapply inv_wtt_ref   in H as [[? ?] | [? ?]]
+  | H : wtt <{new _ : _}> |- _ => eapply inv_wtt_new   in H
+  | H : wtt <{* _      }> |- _ => eapply inv_wtt_load  in H
+  | H : wtt <{_ := _   }> |- _ => eapply inv_wtt_asg   in H as [? ?]
+  | H : wtt <{acq _ _  }> |- _ => eapply inv_wtt_acq   in H as [? ?]
+  | H : wtt <{cr _ _   }> |- _ => eapply inv_wtt_cr    in H
+  | H : wtt <{ptm _ _  }> |- _ => eapply inv_wtt_ptm   in H
+  | H : wtt <{spawn _  }> |- _ => eapply inv_wtt_spawn in H
+  end.
+
